Notations

theories/lr_lemma.v
@@ -13,26 +13,29 @@ From iris.base_logic Require Import invariants.
 
 Section Sec.
   Context `{HdotG: dotG Σ}.
-  Definition vstp Γ T1 T2 := ∀ v ρ, interp_env Γ ρ -> interp T1 ρ v -> interp T2 ρ v.
-  Definition ivstp Γ T1 T2: iProp Σ := (□∀ v ρ, interp_env Γ ρ -∗ interp T1 ρ v -∗ interp T2 ρ v)%I.
+  Definition vstp Γ T1 T2 := ∀ v ρ, ⟦Γ⟧* ρ -> ⟦T1⟧ ρ v -> ⟦T2⟧ ρ v.
+  Definition ivstp Γ T1 T2: iProp Σ := (□∀ v ρ, ⟦Γ⟧* ρ -∗ ⟦T1⟧ ρ v -∗ ⟦T2⟧ ρ v)%I.
   Arguments vstp /.
   Arguments ivstp /.
+  Notation "Γ ⊨ T1 <: T2" := (ivstp Γ T1 T2) (at level 74, T1, T2 at next level).
+
   Context (Γ: list ty).
+
 
   (* Lemma stp_later T ρ v: interp T ρ v -∗ interp (TLater T) ρ v. *)
   (* Proof. iIntros; by iNext. Qed. *)
-  Lemma ivstp_later T: ivstp Γ T (TLater T).
+  Lemma ivstp_later G T: G ⊨ T <: TLater T.
   Proof. iIntros "!> ** /="; by iNext. Qed.
 
-  Lemma ivstp_ande1 T1 T2: ivstp Γ (TAnd T1 T2) T1.
+  Lemma ivstp_ande1 T1 T2: Γ ⊨ TAnd T1 T2 <: T1.
   Proof. by iIntros "/= !> * ? [? ?]". Qed.
-  Lemma ivstp_ande2 T1 T2: ivstp Γ (TAnd T1 T2) T2.
+  Lemma ivstp_ande2 T1 T2: Γ ⊨ TAnd T1 T2 <: T2.
   Proof. by iIntros "/= !> * ? [? ?]". Qed.
 
   Lemma stp_andi T1 T2 ρ v:
-    interp T1 ρ v -∗
-    interp T2 ρ v -∗
-    interp (TAnd T1 T2) ρ v.
+    ⟦T1⟧ ρ v -∗
+    ⟦T2⟧ ρ v -∗
+    ⟦TAnd T1 T2⟧ ρ v.
   Proof. iIntros; by iSplit. Qed.
 
   Lemma vstp_andi S T1 T2:
@@ -42,36 +45,37 @@ Section Sec.
   Proof. move => /= H1 H2 v ρ Hg HS; by iSplit; [iApply H1 | iApply H2]. Qed.
 
   Lemma ivstp_andi S T1 T2:
-    ivstp Γ S T1 -∗
-    ivstp Γ S T2 -∗
-    ivstp Γ S (TAnd T1 T2).
+    Γ ⊨ S <: T1 -∗
+    Γ ⊨ S <: T2 -∗
+    Γ ⊨ S <: TAnd T1 T2.
   Proof.
     iIntros "/= #H1 #H2 !> * #Hg #HS".
     iApply stp_andi; [iApply "H1" | iApply "H2"]; done.
   Qed.
 
-  Lemma stp_ori1 T1 T2 ρ v: interp T1 ρ v -∗ interp (TOr T1 T2) ρ v.
+  Lemma stp_ori1 T1 T2 ρ v: ⟦T1⟧ ρ v -∗ ⟦TOr T1 T2⟧ ρ v.
   Proof. iIntros "? /="; by iLeft. Qed.
-  Lemma stp_ori2 T1 T2 ρ v: interp T2 ρ v -∗ interp (TOr T1 T2) ρ v.
+  Lemma stp_ori2 T1 T2 ρ v: ⟦T2⟧ ρ v -∗ ⟦TOr T1 T2⟧ ρ v.
   Proof. iIntros "? /="; by iRight. Qed.
 
   Lemma ivstp_ore S T1 T2:
-    ivstp Γ T1 S -∗
-    ivstp Γ T2 S -∗
-    ivstp Γ (TOr T1 T2) S.
+    Γ ⊨ T1 <: S -∗
+    Γ ⊨ T2 <: S -∗
+    Γ ⊨ TOr T1 T2 <: S.
   Proof. iIntros "/= #H1 #H2 !> * #Hg #[HT1 | HT2]"; [iApply "H1" | iApply "H2"]; done. Qed.
 
-  Lemma ivstp_ori1 T1 T2: ivstp Γ T1 (TOr T1 T2).
+  Lemma ivstp_ori1 T1 T2: Γ ⊨ T1 <: TOr T1 T2.
   Proof. iIntros "!> ** /="; by iLeft. Qed.
-  Lemma ivstp_ori2 T1 T2: ivstp Γ T2 (TOr T1 T2).
+  Lemma ivstp_ori2 T1 T2: Γ ⊨ T2 <: TOr T1 T2.
   Proof. iIntros "!> ** /="; by iRight. Qed.
 
-  Definition ivtp Γ T v: iProp Σ := (□∀ ρ, interp_env Γ ρ -∗ interp T ρ v)%I.
+  Definition ivtp Γ T v : iProp Σ := (□∀ ρ, ⟦Γ⟧* ρ -∗ ⟦T⟧ ρ v)%I.
+
   Arguments ivtp /.
 
   Lemma mem_stp_sela_sub L U va l:
     ivtp Γ (TTMem l L U) va -∗
-    ivstp Γ L (TSelA (pv va) l L U).
+    Γ ⊨ L <: TSelA (pv va) l L U.
   Proof.
     iIntros "/= #Hva !>" (v ρ) "#Hg #HvL !>".
     iPoseProof ("Hva" $! ρ with "Hg") as (ϕ) "#[Hlookup [HLϕ HϕU]]"; iClear "Hva".
